PR review

CoqOfRust/revm/links/dependencies.v
@@ -2,249 +2,9 @@ Require Import CoqOfRust.CoqOfRust.
 Require Import CoqOfRust.links.M.
 Require Import core.convert.links.mod.
 Require Import core.links.array.
-Require Import core.ops.links.range.
 Require Import core.links.clone.
 Require Import core.links.default.
 Require Import ruint.links.lib.
-
-(* 
-TODO: 
-- Start link with beneficiary's Address return type
-- In `beneficiary`, link it to Address type(?)
-- Link Addesss::into_word
-- Link Uint::into
-*)
-
-Module alloy_primitives.
-  Module bits.
-    Module links.
-      Module fixed.
-        (* pub struct FixedBytes<const N: usize>(#[into_iterator(owned, ref, ref_mut)] pub [u8; N]); *)
-        Module FixedBytes.
-          Parameter t : Usize.t -> Set.
-
-          Parameter to_value : forall {N : Usize.t}, t N -> Value.t.
-
-          Global Instance IsLink {N : Usize.t} : Link (t N) := {
-            Φ := Ty.apply (Ty.path "alloy_primitives::bits::fixed::FixedBytes") [ φ N ] [];
-            φ := to_value;
-          }.
-
-          Definition of_ty (N : Usize.t) (N' : Value.t) :
-            N' = φ N ->
-            OfTy.t (Ty.apply (Ty.path "alloy_primitives::bits::fixed::FixedBytes") [ N' ] []).
-          Proof.
-            intros.
-            eapply OfTy.Make with (A := t N).
-            now subst.
-          Defined.
-          Smpl Add eapply of_ty : of_ty.
-        End FixedBytes.
-
-        Module Impl_From_for_FixedBytes.
-          Definition Self (N : Usize.t) : Set :=
-            FixedBytes.t N.
-
-          Parameter from : forall (N : Usize.t), PolymorphicFunction.t.
-
-          Axiom Implements :
-            forall (N : Usize.t),
-            M.IsTraitInstance
-              "core::convert::From"
-              (* Trait polymorphic consts *) []
-              (* Trait polymorphic types *) [ Φ (array.t U8.t N) ]
-              (Φ (Self N))
-              (* Instance *) [ ("from", InstanceField.Method (from N)) ].
-
-          Parameter run :
-            forall (N : Usize.t),
-            core.convert.links.mod.From.Run (Self N) (T := array.t U8.t N).
-        End Impl_From_for_FixedBytes.
-        
-        Module Impl_Into_for_FixedBytes.
-          Definition Self (N : Usize.t) : Set :=
-            FixedBytes.t N.
-                  
-          (* fn into(self) -> Uint *)
-          Parameter into : forall (N : Usize.t), PolymorphicFunction.t.
-
-          Axiom Implements :
-            forall (N : Usize.t),
-            M.IsTraitInstance
-              "core::convert::Into" [] [ Φ (array.t U8.t N) ] (Φ (Self N))
-              [ ("into", InstanceField.Method (into N)) ].
-
-          Parameter run :
-            forall (N : Usize.t),
-            core.convert.links.mod.Into.Run (Self N) (array.t U8.t N).
-        End Impl_Into_for_FixedBytes.
-      End fixed.
-
-      Module address.
-        Module Address.
-          Parameter t : Set.
-
-          Parameter to_value : t -> Value.t.
-
-          Global Instance IsLink : Link t := {
-            Φ := Ty.path "alloy_primitives::bits::address::Address";
-            φ := to_value;
-          }.
-
-          Definition of_ty : OfTy.t (Ty.path "alloy_primitives::bits::address::Address").
-          Proof. eapply OfTy.Make with (A := t); reflexivity. Defined.
-          Smpl Add apply of_ty : of_ty.
-        End Address.
-
-        (* impl Address { *)
-        Module Impl_Address.
-          Definition Self : Set :=
-            Address.t.
-
-          (* pub fn from_word(word: FixedBytes<32>) -> Self *)
-          Parameter from_word : PolymorphicFunction.t.
-
-          Global Instance AssociatedFunction_from_word :
-            M.IsAssociatedFunction.Trait (Φ Self) "from_word" from_word.
-          Admitted.
-
-          Global Instance run_from_word (word : fixed.FixedBytes.t {| Integer.value := 32 |}) :
-            Run.Trait from_word [] [] [ φ word ] Address.t.
-          Admitted.
-
-          (* pub fn into_word(&self) -> FixedBytes<32> *)
-          Parameter into_word : PolymorphicFunction.t.
-
-          Global Instance AssociatedFunction_into_word :
-            M.IsAssociatedFunction.Trait (Φ Self) "into_word" into_word.
-          Admitted.
-
-          Global Instance run_into_word (self : Address.t) :
-            Run.Trait into_word [] [] [ φ self ] (fixed.FixedBytes.t {| Integer.value := 32 |}).
-          Admitted.
-
-        End Impl_Address.
-      End address.
-    End links.
-  End bits.
-
-  Module links.
-    Module bytes_.
-      Module Bytes.
-        Parameter t : Set.
-
-        Parameter to_value : t -> Value.t.
-
-        Global Instance IsLink : Link t := {
-          Φ := Ty.path "alloy_primitives::bytes_::Bytes";
-          φ := to_value;
-        }.
-
-        Definition of_ty : OfTy.t (Ty.path "alloy_primitives::bytes_::Bytes").
-        Proof. eapply OfTy.Make with (A := t); reflexivity. Defined.
-        Smpl Add apply of_ty : of_ty.
-      End Bytes.
-
-      Module Impl_Bytes.
-        Definition Self : Set :=
-          Bytes.t.
-
-        (* pub fn new() -> Self *)
-        Parameter new : PolymorphicFunction.t.
-
-        Global Instance AssociatedFunction_new :
-          M.IsAssociatedFunction.Trait (Φ Self) "new" new.
-        Admitted.
-
-        Global Instance run_new : Run.Trait new [] [] [] Bytes.t.
-        Admitted.
-
-        (* pub fn slice(&self, range: impl RangeBounds<usize>) -> Self *)
-        Parameter slice : PolymorphicFunction.t.
-
-        Global Instance AssociatedFunction_slice :
-          M.IsAssociatedFunction.Trait (Φ Self) "slice" slice.
-        Admitted.
-
-        Global Instance run_slice {A : Set} `{Link A} 
-          (self : Ref.t Pointer.Kind.Ref Self) 
-          (range : A) 
-          (run_RangeBounds_for_A : RangeBounds.Run A) :
-          Run.Trait slice [] [] [φ self; φ range] Self.
-        Admitted.
-      End Impl_Bytes.
-      
-      Module Impl_Clone_for_Bytes.
-        Definition Self : Ty.t := Ty.path "alloy_primitives::bytes_::Bytes".
-
-        Parameter clone : PolymorphicFunction.t.
-
-        Axiom Implements :
-          M.IsTraitInstance
-            "core::clone::Clone"
-            (* Trait polymorphic consts *) []
-            (* Trait polymorphic types *) []
-            Self
-            (* Instance *) [ ("clone", InstanceField.Method clone) ].
-
-        Definition run_clone : clone.Clone.Run_clone Bytes.t.
-        Admitted.
-      
-        Instance run : Clone.Run Bytes.t := {
-          CLone.clone := run_clone;
-        }.
-      End Impl_Clone_for_Bytes.
-
-      Module Impl_Default_for_Bytes.
-        Definition Self : Ty.t := Ty.path "alloy_primitives::bytes_::Bytes".
-
-        Parameter default : PolymorphicFunction.t.
-
-        Axiom Implements :
-          M.IsTraitInstance
-            "default::default::Default"
-            (* Trait polymorphic consts *) []
-            (* Trait polymorphic types *) []
-            Self
-            (* Instance *) [ ("default", InstanceField.Method default) ].
-
-        Definition run_default : default.Default.Run_default Bytes.t.
-        Admitted.
-      
-        Instance run : Default.Run Bytes.t := {
-          Default.default := run_default;
-        }.
-      End Impl_Default_for_Bytes.
-    End bytes_.
-  End links.
-End alloy_primitives.
-
-Module FixedBytes.
-  Parameter t : Set.
-
-  Parameter to_value : t -> Value.t.
-
-  Global Instance IsLink : Link t := {
-    Φ := Ty.path "alloy_primitives::bits::fixed::FixedBytes";
-    φ := to_value;
-  }.
-
-  (* TODO: 
-  - (alloy_primitives::FixedBytes) fn into(self) -> Uint
-  *)
-End FixedBytes.
-
-(** ** Here we define some aliases that are convenient *)
-
-Module U256.
-  Definition t : Set :=
-    Uint.t {| Integer.value := 256 |} {| Integer.value := 4 |}.
-End U256.
-
-Module B256.
-  Definition t : Set :=
-    alloy_primitives.bits.links.fixed.FixedBytes.t {| Integer.value := 32 |}.
-End B256.
 
 Module ruint.
   Module Impl_Uint.
@@ -260,7 +20,7 @@ Module ruint.
 
     Global Instance wrapping_add_IsAssociated :
       forall (BITS LIMBS : Value.t),
-      M.IsAssociatedFunction.Trait
+      M.IsAssociatedFunction.C
         (Self_ty BITS LIMBS)
         "wrapping_add"
         (wrapping_add BITS LIMBS).
@@ -279,7 +39,7 @@ Module ruint.
 
     Global Instance to_be_bytes_IsAssociated :
       forall (BITS LIMBS : Value.t),
-      M.IsAssociatedFunction.Trait
+      M.IsAssociatedFunction.C
         (Self_ty BITS LIMBS)
         "to_be_bytes"
         (to_be_bytes BITS LIMBS).
@@ -305,7 +65,7 @@ Module ruint.
     
     Global Instance bit_IsAssociated :
       forall (BITS LIMBS : Value.t),
-        M.IsAssociatedFunction.Trait
+        M.IsAssociatedFunction.C
           (Self_ty BITS LIMBS)
           "bit"
           (bit BITS LIMBS).
@@ -335,7 +95,7 @@ Module ruint.
     
     Global Instance is_zero_IsAssociated :
       forall (BITS LIMBS : Value.t),
-        M.IsAssociatedFunction.Trait
+        M.IsAssociatedFunction.C
           (Self_ty BITS LIMBS)
           "is_zero"
           (is_zero BITS LIMBS).
@@ -360,7 +120,7 @@ Module ruint.
 
     Global Instance from_IsAssociated :
       forall (BITS LIMBS : Value.t),
-      M.IsAssociatedFunction.Trait
+      M.IsAssociatedFunction.C
         (Self_ty BITS LIMBS)
         "from"
         (from BITS LIMBS).
@@ -606,7 +366,7 @@ Module ruint.
   
     Axiom Implements_AsLimbs :
       forall (BITS LIMBS : Value.t),
-        IsAssociatedFunction.Trait
+        IsAssociatedFunction.C
           (Ty.apply (Ty.path "ruint::Uint") [BITS; LIMBS] [])
           "as_limbs"
           (as_limbs BITS LIMBS).
