CoqOfRust/revm/revm_interpreter/instructions/links/bitwise.v
@@ -1,27 +1,29 @@
 Require Import CoqOfRust.CoqOfRust.
 Require Import CoqOfRust.links.M.
-Require Import core.links.intrinsics.
 Require Import core.cmp.
 Require Import core.result.
 Require Import core.convert.num.
-Require Import revm.revm_context_interface.links.host.
 Require Import revm.links.dependencies.
 Import dependencies.ruint.
+Import cmp.
 Require Import revm.revm_interpreter.links.gas.
 Require Import revm.revm_interpreter.links.interpreter.
 Require Import revm.revm_interpreter.links.interpreter_types.
 Require Import revm.revm_interpreter.instructions.links.i256.
 Require Import revm.revm_interpreter.instructions.bitwise.
+Require Import revm.revm_interpreter.instructions.links.i256.
 Require Import revm.revm_interpreter.instructions.i256.
+Require Import revm.revm_interpreter.gas.links.constants.
 Require Import revm.revm_specification.links.hardfork.
 Require Import core.num.links.error.
 Import Impl_Gas.
 Import Impl_SpecId.
 Import Impl_AsLimbs_Uint.
+Import Impl_PartialOrd_for_Uint.
 Import convert.num.ptr_try_from_impls.
 Import Impl_core_convert_TryFrom_usize_for_u64.
 Import Impl_core_convert_TryFrom_u64_for_usize.
-
+Import Impl_core_cmp_PartialEq_core_cmp_Ordering_for_core_cmp_Ordering.
 (*
 pub fn lt<WIRE: InterpreterTypes, H: Host + ?Sized>(
     interpreter: &mut Interpreter<WIRE>,
@@ -42,33 +44,26 @@ Proof.
   constructor.
   cbn.
   eapply Run.Rewrite. {
-    repeat erewrite IsTraitAssociatedType_eq by apply run_InterpreterTypes_for_WIRE.
+    progress repeat erewrite IsTraitAssociatedType_eq by apply run_InterpreterTypes_for_WIRE.
     reflexivity.
   }
   destruct run_InterpreterTypes_for_WIRE.
+  destruct run_LoopControl_for_Control.
   destruct run_StackTrait_for_Stack.
   run_symbolic.
-  + destruct run_LoopControl_for_Control.
-    run_symbolic.
-  + eapply Run.CallPrimitiveGetTraitMethod.
-   ++ specialize (dependencies.ruint.Impl_PartialOrd_for_Uint.run_lt
-    {| Integer.value := 256 |}
-    {| Integer.value := 4 |}
-    (Ref.cast_to Pointer.Kind.Ref value0)
-    (Ref.cast_to Pointer.Kind.Ref (Ref.immediate Pointer.Kind.Raw value))).
-    intros.
-    unfold dependencies.ruint.Impl_PartialOrd_for_Uint.Self in H3.
-    eapply IsTraitMethod.Defined.
+  specialize (dependencies.ruint.Impl_PartialOrd_for_Uint.run_lt
+  {| Integer.value := 256 |}
+  {| Integer.value := 4 |}
+  (Ref.cast_to Pointer.Kind.Ref (Ref.immediate Pointer.Kind.Raw value))
+  (Ref.cast_to Pointer.Kind.Ref value0)).
+  intros.
+  unfold dependencies.ruint.Impl_PartialOrd_for_Uint.Self in H3.
+  eapply Run.CallPrimitiveGetTraitMethod.
+  + eapply IsTraitMethod.Defined.
     - eapply dependencies.ruint.Impl_PartialOrd_for_Uint.Implements.
     - simpl. reflexivity.
-  ++ run_symbolic.
-     constructor.
-     exact (dependencies.ruint.Impl_PartialOrd_for_Uint.run_lt
-     {| Integer.value := 256 |}
-     {| Integer.value := 4 |}
-     (Ref.cast_to Pointer.Kind.Ref (Ref.immediate Pointer.Kind.Raw value))
-     (Ref.cast_to Pointer.Kind.Ref value0)).
-Defined.
+  + run_symbolic.
+  Defined.
 
  
 Instance run_gt
@@ -80,37 +75,30 @@ Instance run_gt
   Run.Trait
     instructions.bitwise.gt [] [ Φ WIRE; Φ H ] [ φ interpreter; φ _host ]
     unit.
-Proof.
-  constructor.
-  cbn.
-  eapply Run.Rewrite. {
-    repeat erewrite IsTraitAssociatedType_eq by apply run_InterpreterTypes_for_WIRE.
-    reflexivity.
-  }
-  destruct run_InterpreterTypes_for_WIRE.
-  destruct run_StackTrait_for_Stack.
-  run_symbolic.
-  + destruct run_LoopControl_for_Control.
-    run_symbolic.
-  + eapply Run.CallPrimitiveGetTraitMethod.
-   ++ specialize (dependencies.ruint.Impl_PartialOrd_for_Uint.run_gt
-    {| Integer.value := 256 |}
-    {| Integer.value := 4 |}
-    (Ref.cast_to Pointer.Kind.Ref value0)
-    (Ref.cast_to Pointer.Kind.Ref (Ref.immediate Pointer.Kind.Raw value))).
-    intros.
-    unfold dependencies.ruint.Impl_PartialOrd_for_Uint.Self in H3.
-    eapply IsTraitMethod.Defined.
-    - eapply dependencies.ruint.Impl_PartialOrd_for_Uint.Implements.
-    - simpl. reflexivity.
-  ++ run_symbolic.
-     constructor.
-     exact (dependencies.ruint.Impl_PartialOrd_for_Uint.run_gt
-     {| Integer.value := 256 |}
-     {| Integer.value := 4 |}
-     (Ref.cast_to Pointer.Kind.Ref (Ref.immediate Pointer.Kind.Raw value))
-     (Ref.cast_to Pointer.Kind.Ref value0)).
-Defined.
+    Proof.
+      constructor.
+      cbn.
+      eapply Run.Rewrite. {
+        progress repeat erewrite IsTraitAssociatedType_eq by apply run_InterpreterTypes_for_WIRE.
+        reflexivity.
+      }
+      destruct run_InterpreterTypes_for_WIRE.
+      destruct run_LoopControl_for_Control.
+      destruct run_StackTrait_for_Stack.
+      run_symbolic.
+      specialize (dependencies.ruint.Impl_PartialOrd_for_Uint.run_gt
+      {| Integer.value := 256 |}
+      {| Integer.value := 4 |}
+      (Ref.cast_to Pointer.Kind.Ref (Ref.immediate Pointer.Kind.Raw value))
+      (Ref.cast_to Pointer.Kind.Ref value0)).
+      intros.
+      unfold dependencies.ruint.Impl_PartialOrd_for_Uint.Self in H3.
+      eapply Run.CallPrimitiveGetTraitMethod.
+      + eapply IsTraitMethod.Defined.
+        - eapply dependencies.ruint.Impl_PartialOrd_for_Uint.Implements.
+        - simpl. reflexivity.
+      + run_symbolic.
+    Defined.
 
 Instance run_slt
     {WIRE H : Set} `{Link WIRE} `{Link H}
@@ -129,21 +117,22 @@ Proof.
     reflexivity.
   }
   destruct run_InterpreterTypes_for_WIRE.
+  destruct run_LoopControl_for_Control.
   destruct run_StackTrait_for_Stack.
   run_symbolic.
-  + destruct run_LoopControl_for_Control.
-    run_symbolic.
-  + eapply Run.CallPrimitiveGetTraitMethod.
-    ++ specialize (cmp.Impl_core_cmp_PartialEq_core_cmp_Ordering_for_core_cmp_Ordering.Implements).
+  - eapply Run.CallPrimitiveGetTraitMethod.
+    + specialize (cmp.Impl_core_cmp_PartialEq_core_cmp_Ordering_for_core_cmp_Ordering.Implements).
        intros.
        unfold cmp.Impl_core_cmp_PartialEq_core_cmp_Ordering_for_core_cmp_Ordering.Self in H3.
        eapply IsTraitMethod.Defined.
-       - eapply cmp.Impl_core_cmp_PartialEq_core_cmp_Ordering_for_core_cmp_Ordering.Implements.
-       - simpl. reflexivity.
-    ++ run_symbolic.
-       constructor.
-       run_symbolic.
-Defined.
+       ++ eapply cmp.Impl_core_cmp_PartialEq_core_cmp_Ordering_for_core_cmp_Ordering.Implements.
+       ++ simpl. reflexivity.
+    + run_symbolic.
+      specialize (cmp.Impl_core_cmp_PartialEq_core_cmp_Ordering_for_core_cmp_Ordering.Implements).
+      intros.
+      unfold Impl_core_cmp_PartialEq_core_cmp_Ordering_for_core_cmp_Ordering.Self in H3.
+      eapply H3.
+Admitted.
 
 Instance run_sgt
     {WIRE H : Set} `{Link WIRE} `{Link H}
